More work on event proof

example/event.go
@@ -6,8 +6,8 @@ import (
 
 type Event struct {
 	id    uint32
-	start TimeStamp
-	end   TimeStamp
+	start *TimeStamp
+	end   *TimeStamp
 }
 
 func MarshalEvent(e *Event) []byte {
@@ -15,8 +15,8 @@ func MarshalEvent(e *Event) []byte {
 	// How important is knowing the capacity in the first place?
 	var enc = make([]byte, 0, 28)
 	enc = marshal.WriteInt32(enc, e.id)
-	enc = marshal.WriteBytes(enc, MarshalTimeStamp(&e.start))
-	enc = marshal.WriteBytes(enc, MarshalTimeStamp(&e.end))
+	enc = marshal.WriteBytes(enc, MarshalTimeStamp(e.start))
+	enc = marshal.WriteBytes(enc, MarshalTimeStamp(e.end))
 	return enc
 }
 
@@ -24,8 +24,8 @@ func UnmarshalEvent(s []byte) *Event {
 	e := new(Event)
 	var enc = s // Needed for goose compatibility
 	e.id, enc = marshal.ReadInt32(enc)
-	e.start = *UnmarshalTimeStamp(enc[:12])
+	e.start = UnmarshalTimeStamp(enc[:12])
 	enc = enc[12:]
-	e.end = *UnmarshalTimeStamp(enc[:12])
+	e.end = UnmarshalTimeStamp(enc[:12])
 	return e
 }
