example/event_marshal_proof.v
@@ -11,20 +11,22 @@ Context `{!heapGS Σ}.
 Record EventStruct :=
   mkC {
       id : u32 ;
-      startTime : list u8 ;
-      endTime : list u8 ;
+      startTime : encodeTimestamp.Timestamp ;
+      endTime : encodeTimestamp.Timestamp ;
     }.
 
+Search loc.
+
 Definition has_encoding (encoded:list u8) (args:EventStruct) : Prop :=
-  encoded = (u32_le args.(id)) ++ args.(startTime) ++ args.(endTime).
+  encoded = (u32_le args.(id)) ++ (encodeTimestamp.wp_Encode args.(startTime)) ++ args.(endTime).
 
 Definition own args_ptr args q : iProp Σ :=
   ∃ start_sl end_sl,
   "Hargs_id" ∷ args_ptr ↦[Event :: "id"]{q} #args.(id) ∗
-  "Hargs_start" ∷ args_ptr ↦[Event :: "startTime"]{q} (slice_val start_sl) ∗
-  "Hargs_start_sl" ∷ own_slice_small start_sl byteT q args.(startTime) ∗
-  "Hargs_end" ∷ args_ptr ↦[Event :: "endTime"]{q} (slice_val end_sl) ∗
-  "Hargs_end_sl" ∷ own_slice_small end_sl byteT q args.(endTime).
+  "Hargs_start" ∷ args_ptr ↦[Event :: "startTimeBin"]{q} (slice_val start_sl) ∗
+  "Hargs_start_sl" ∷ own_slice_small start_sl byteT q args.(startTimeBin) ∗
+  "Hargs_end" ∷ args_ptr ↦[Event :: "endTimeBin"]{q} (slice_val end_sl) ∗
+  "Hargs_end_sl" ∷ own_slice_small end_sl byteT q args.(endTimeBin).
 
 Lemma wp_Encode (args_ptr:loc) (args:EventStruct) :
   {{{
@@ -50,8 +52,8 @@ Proof.
 
   wp_apply (wp_struct_fieldRef). { done. }
   wp_apply (encodeTimestamp.wp_Encode with "[Hargs_start Hargs_start_sl]").
-  - unfold encodeTimestamp.own.
-Admitted.
+  - unfold encodeTimestamp.own. Search (_ -> loc).
+Abort.
 
 Lemma wp_Decode enc enc_sl (args:EventStruct) :
   {{{
@@ -63,7 +65,7 @@ Lemma wp_Decode enc enc_sl (args:EventStruct) :
         args_ptr, RET #args_ptr; own args_ptr args (DfracOwn 1)
   }}}.
 Proof.
-  Admitted.
+  Abort.
 
 End encodeEvent.
 End encodeEvent.
