go.mod
@@ -4,6 +4,9 @@ go 1.22.5
 
 require github.com/goose-lang/primitive v0.1.0 // indirect
 
-require github.com/tchajed/marshal v0.6.2
+require (
+	github.com/tchajed/marshal v0.6.2
+	google.golang.org/protobuf v1.34.2
+)
 
 require github.com/goose-lang/std v0.4.1 // indirect
